GenericModuleLib/Concept1.v
@@ -1,0 +1,404 @@
+(* %%%%%%%%%%%%%%%%%%%%%%%%%%%%%%%%%%%%%%%%%%%%%%%%%%%%%%%%%%%%%%%%% *) 
+(* Module
+  
+   Last Update: Fri, 28 Apr 2017
+ %%%%%%%%%%%%%%%%%%%%%%%%%%%%%%%%%%%%%%%%%%%%%%%%%%%%%%%%%%%%%%%%%%% *) 
+
+Add LoadPath "../..".
+
+Require Import ConceptParams.AuxTactics.LibTactics.
+Require Import ConceptParams.AuxTactics.BasicTactics.
+
+Require Import ConceptParams.List2AVL.List2Set.
+
+Require Import Coq.Lists.List.
+Import ListNotations.
+Require Import Coq.Bool.Bool.
+
+Require Import Coq.Structures.Orders.
+
+(* ***************************************************************** *)
+(** * TODO 
+
+      (TODO) *)
+
+(** TODO *)
+(* ***************************************************************** *)
+(* ***************************************************************** *)
+
+(* ################################################################# *)
+(** ** TODO *)
+(* ################################################################# *)
+
+Module Type Typ.
+  Parameter t : Type.
+  Parameter ctx : Type.
+End Typ.
+
+Module Type TypOkDef (Import T : Typ).
+  Parameter is_ok : ctx -> t -> Prop.
+End TypOkDef.
+
+Module Type TypOkInterp (Import T : Typ).
+  Parameter is_ok_b : ctx -> t -> bool.
+End TypOkInterp.
+
+Module Type TypOkProp (Import T : Typ) 
+       (Import TD : TypOkDef T) (Import TI : TypOkInterp T).
+
+  Axiom is_ok_b__sound : forall (c : ctx) (x : t),
+      is_ok_b c x = true -> is_ok c x.
+  Axiom is_ok_b__complete : forall (c : ctx) (x : t),
+      is_ok c x -> is_ok_b c x = true.
+End TypOkProp.
+
+
+Module Type Concept1Base.
+  Declare Module IdOT : UsualOrderedType.
+  Declare Module TyTP : Typ.
+  Declare Module IdLS : List2Set IdOT.
+
+  Definition id := IdOT.t.
+  Definition ty := TyTP.t.
+  Definition ctx := TyTP.ctx.
+End Concept1Base.
+
+
+Module MConcept1Defs (Import MCB : Concept1Base) 
+       (Import TOkD : TypOkDef MCB.TyTP).
+
+  Definition types_ok (c : ctx) (tps : list ty) : Prop :=
+    List.Forall (fun tp => is_ok c tp) tps.
+
+  Definition concept_ok (c : ctx) (ds : list (id * ty)) : Prop :=
+    let (nms, tps) := split ds in
+    (** all names are distinct *)
+    List.NoDup nms
+    (** and all types are valid *)
+    /\ types_ok c tps. 
+
+End MConcept1Defs.
+
+
+Module MConcept1Interp (Import MCB : Concept1Base) 
+       (Import TOkI : TypOkInterp MCB.TyTP).
+
+  Definition types_ok_b (c : ctx) (tps : list ty) : bool :=
+    List.forallb (fun tp => is_ok_b c tp) tps.
+
+  Definition concept_ok_b (c : ctx) (ds : list (id * ty)) : bool :=
+    let (nms, tps) := split ds in
+    andb
+      (** all names are distinct *)
+      (IdLS.ids_are_unique nms)
+      (** and all types are valid *)
+      (types_ok_b c tps).
+ 
+End MConcept1Interp.
+
+
+Module MConcept1Props 
+       (Import MCB : Concept1Base)
+       (Import TOkD : TypOkDef MCB.TyTP)
+       (Import TOkI : TypOkInterp MCB.TyTP)
+       (Import TOkP : TypOkProp MCB.TyTP TOkD TOkI)
+.
+  Module Import MCD := MConcept1Defs   MCB TOkD.
+  Module Import MCI := MConcept1Interp MCB TOkI.
+
+  Lemma types_ok_b__sound : forall (c : ctx) (ts : list ty),
+      types_ok_b c ts = true ->
+      types_ok c ts.
+  Proof.
+    intros c ts. unfold types_ok_b.
+    induction ts as [| tp ts'];
+      intros H.
+    - (* ts = nil *)
+      apply Forall_nil.
+    - (* ts = tp :: ts' *)
+      simpl in H. rewrite -> andb_true_iff in H.
+      inversion H as [Htp Hts']; clear H.
+      apply IHts' in Hts'. 
+      apply TOkP.is_ok_b__sound in Htp.
+      apply Forall_cons; auto.
+  Qed.
+
+  Lemma types_ok_b__complete : forall (c : ctx) (ts : list ty),
+      types_ok c ts ->
+      types_ok_b c ts = true.
+  Proof.
+    intros c ts. unfold types_ok_b.
+    induction ts as [| tp ts' IHts'];
+      intros H.
+    - (* ts = nil *)
+      reflexivity.
+    - (* ts = tp :: ts' *)
+      inversion H; subst.
+      simpl. rewrite -> andb_true_iff. split.
+      + apply TOkP.is_ok_b__complete. assumption.
+      + apply IHts'. assumption.
+  Qed.
+
+  Lemma concept_ok_b__sound : forall (c : ctx) (ds : list (id * ty)),
+      concept_ok_b c ds = true ->
+      concept_ok c ds.
+  Proof.
+    intros c ds. intros H.
+    unfold concept_ok_b in H. 
+    unfold concept_ok.
+    destruct (split ds).
+    rewrite -> andb_true_iff in H. inversion H as [Hid Hty].
+    apply IdLS.Props.ids_are_unique__sound in Hid.
+    apply types_ok_b__sound in Hty.
+    split; tauto.
+  Qed.
+
+  Lemma concept_ok_b__complete : forall (c : ctx) (ds : list (id * ty)),
+      concept_ok c ds ->
+      concept_ok_b c ds = true.
+  Proof.
+    intros c ds. intros H.
+    unfold concept_ok_b.
+    unfold concept_ok in H.
+    destruct (split ds).
+    inversion H as [Hdup Htys].
+    rewrite -> andb_true_iff. split.
+    apply IdLS.Props.ids_are_unique__complete in Hdup. assumption.
+    apply types_ok_b__complete. assumption.
+  Qed.
+
+End MConcept1Props.
+
+
+
+
+
+
+
+
+
+
+
+
+
+
+
+
+(*
+Module Type HasWellDef <: Typ.
+
+  Include Typ.
+
+  Parameter is_welldef   : t -> Prop.
+  Parameter is_welldef_b : t -> bool.
+
+End HasWellDef.
+
+
+Module Type Concept1Base.
+
+  Declare Module IdOT : UsualOrderedType.
+  Declare Module TyWD : HasWellDef.
+  Declare Module IdLS : List2Set IdOT.
+
+  Definition id := IdOT.t.
+  Definition ty := TyWD.t.
+
+End Concept1Base.
+
+Module Type Concept1Defs (Import MCB : Concept1Base).
+
+  Parameter types_ok : list ty -> Prop.
+  Parameter concept_ok : list (id * ty) -> Prop.
+
+End Concept1Defs.
+
+Module Type Concept1Interp (Import MCB : Concept1Base).
+
+  Parameter types_ok_b : list ty -> bool.
+  Parameter concept_ok_b : list (id * ty) -> bool.
+
+End Concept1Interp.
+
+
+Module MConcept1Base
+       (id_UOT : UsualOrderedType)
+       (ty_WD  : HasWellDef)
+       (id_LS  : List2Set id_UOT)
+<: Concept1Base.
+
+  Module IdOT := id_UOT.
+  Module TyWD := ty_WD.
+  Module IdLS := id_LS.
+
+  Definition id := IdOT.t.
+  Definition ty := TyWD.t.
+
+End MConcept1Base.
+
+
+Module MConcept1Defs (Import MCB : Concept1Base).
+
+  Definition types_ok (tps : list ty) : Prop :=
+    List.Forall (fun tp => TyWD.is_welldef tp) tps.
+
+  Definition concept_ok (ds : list (id * ty)) : Prop :=
+    let (nms, tps) := split ds in
+    (** all names are distinct *)
+    List.NoDup nms
+    (** and all types are valid *)
+    /\ types_ok tps. 
+
+End MConcept1Defs.
+
+
+Module MConcept1Interp (Import MCB : Concept1Base).
+
+  Definition types_ok_b (tps : list ty) : bool :=
+    List.forallb (fun tp => TyWD.is_welldef_b tp) tps.
+
+  Definition concept_ok_b (ds : list (id * ty)) : bool :=
+    let (nms, tps) := split ds in
+    andb
+      (** all names are distinct *)
+      (IdLS.ids_are_unique nms)
+      (** and all types are valid *)
+      (types_ok_b tps).
+ 
+End MConcept1Interp.
+
+
+Module MConcept1Props 
+       (Import MCB : Concept1Base)
+.
+  Module Import MCD := MConcept1Defs   MCB.
+  Module Import MCI := MConcept1Interp MCB.
+
+  Lemma types_ok_b__sound : forall (ts : list ty),
+        types_ok_b ts = true ->
+        types_ok ts.
+    Proof.
+      intros ts. unfold types_ok_b.
+      induction ts as [| tp ts'];
+        intros H.
+      - (* ts = nil *)
+        apply Forall_nil.
+      - (* ts = tp :: ts' *)
+        simpl in H. rewrite -> andb_true_iff in H.
+        inversion H as [Htp Hts']; clear H.
+        apply IHts' in Hts'. 
+        apply TyWD.is_welldef_b__sound in Htp.
+        apply Forall_cons; auto.
+    Qed.
+
+    Lemma types_ok_b__complete : forall (ts : list ty),
+        types_ok ts ->
+        types_ok_b ts = true.
+    Proof.
+      intros ts. unfold types_ok_b.
+      induction ts as [| tp ts' IHts'];
+        intros H.
+      - (* ts = nil *)
+        reflexivity.
+      - (* ts = tp :: ts' *)
+        inversion H; subst.
+        simpl. rewrite -> andb_true_iff. split.
+        + apply TyWD.is_welldef_b__complete. assumption.
+        + apply IHts'. assumption.
+    Qed.
+
+End MConcept1Props.
+
+(*
+Module MConcept1 
+       (id_UOT : UsualOrderedType)
+       (ty_WD  : HasWellDef)
+       (id_LS  : List2Set id_UOT)
+.
+
+  Module IdOT := id_UOT.
+  Module TyWD := ty_WD.
+  Module IdLS := id_LS.
+
+  Definition id := IdOT.t.
+  Definition ty := TyWD.t.
+
+  (*
+  Definition get_ids (xs : list (id * ty)) : list id 
+      := List.map fst xs.
+  *)
+
+(*  Module PropDefs. *)
+  
+    Definition types_ok (tps : list ty) : Prop :=
+      List.Forall (fun tp => TyWD.is_welldef tp) tps.
+
+    Definition concept_ok (ds : list (id * ty)) : Prop :=
+      let (nms, tps) := split ds in
+      (** all names are distinct *)
+      List.NoDup nms
+      (** and all types are valid *)
+      /\ types_ok tps.    
+
+(*  End PropDefs. *)
+
+
+(*  Module FunDefs. *)
+
+    Definition types_ok_b (tps : list ty) : bool :=
+      List.forallb (fun tp => TyWD.is_welldef_b tp) tps.
+
+    Definition concept_ok_b (ds : list (id * ty)) : bool :=
+      let (nms, tps) := split ds in
+      andb
+        (** all names are distinct *)
+        (IdLS.ids_are_unique nms)
+        (** and all types are valid *)
+        (types_ok_b tps).    
+
+(*  End FunDefs. *)
+
+
+(*  Module Props.
+    Import PropDefs.
+    Import FunDefs. *)
+    
+    Lemma types_ok_b__sound : forall (ts : list ty),
+        types_ok_b ts = true ->
+        types_ok ts.
+    Proof.
+      intros ts. unfold types_ok_b.
+      induction ts as [| tp ts'];
+        intros H.
+      - (* ts = nil *)
+        apply Forall_nil.
+      - (* ts = tp :: ts' *)
+        simpl in H. rewrite -> andb_true_iff in H.
+        inversion H as [Htp Hts']; clear H.
+        apply IHts' in Hts'. 
+        apply TyWD.is_welldef_b__sound in Htp.
+        apply Forall_cons; auto.
+    Qed.
+
+    Lemma types_ok_b__complete : forall (ts : list ty),
+        types_ok ts ->
+        types_ok_b ts = true.
+    Proof.
+      intros ts. unfold types_ok_b.
+      induction ts as [| tp ts' IHts'];
+        intros H.
+      - (* ts = nil *)
+        reflexivity.
+      - (* ts = tp :: ts' *)
+        inversion H; subst.
+        simpl. rewrite -> andb_true_iff. split.
+        + apply TyWD.is_welldef_b__complete. assumption.
+        + apply IHts'. assumption.
+    Qed.
+
+(*  End Props. *)
+
+  
+End MConcept1.
+*)
+*)
